VerifiedFilter/Grammar/KatydidExamples.lean
@@ -166,11 +166,8 @@ open Pred.AnyEq
 
 def example_grammar_doc: Grammar 3 (Pred String) :=
   Grammar.mk (start := Regex.symbol (Pred.eq "doc", 0))
-    (prods := #v[
-      Regex.oneOrMore (Regex.symbol (Pred.eq "p", 1)),
-      Regex.symbol (Pred.any, 2),
-      Regex.emptystr,
-    ])
+    (prods := #v[Regex.oneOrMore (Regex.symbol (Pred.eq "p", 1)),
+      Regex.symbol (Pred.any, 2), Regex.emptystr])
 
 #guard validate example_grammar_doc Pred.evalb
   [node "doc" [node "p" [node "pcdata" []]]]
@@ -299,8 +296,7 @@ def complex: Grammar 7 (Pred String) :=
   mk (interleave (eq ("Due", 1)) (interleave (eq ("Loc", 5)) starAny)) #v[emptystr,
     or (field ("Year", 2)) (and (field ("Year", 3)) (field ("Month", 4))),
     eq ("2026", 0), eq ("2025", 0), symbol (Pred.ge "10", 0),
-    field ("Cont", 6), eq ("EU", 0),
-  ]
+    field ("Cont", 6), eq ("EU", 0)]
 
 #guard validate complex Pred.evalb
   [
