VerifiedFilter/Grammar/Memoize/StateMemoizeExamples.lean
@@ -41,8 +41,7 @@ def complex : Grammar 7 (Pred.Compare.Pred String) :=
   Grammar.mk (interleave (eq ("Due", 1)) (interleave (eq ("Loc", 5)) starAny)) #v[emptystr,
     or (field ("Year", 2)) (and (field ("Year", 3)) (field ("Month", 4))),
     eq ("2026", 0), eq ("2025", 0), symbol (Pred.Compare.Pred.ge "10", 0),
-    field ("Cont", 6), eq ("EU", 0),
-  ]
+    field ("Cont", 6), eq ("EU", 0)]
 
 private def itp_2026 :=
   [
