VerifiedFilter/Parser/HedgeParser.lean
@@ -306,6 +306,8 @@ def runs (x: HedgeParser α β) (h: Hedge α): Bool :=
   | Except.error _ => false
   | Except.ok _ => true
 
+open Token
+
 def exampleParse1 [p: Parser m Token] [MonadExcept String m] [Monad m]: m Unit := do
   assertEq Hint.enter (← p.next) -- enter Hedge.Node
   assertEq Hint.value (← p.next); assertEq (Token.string "blogpost") (← p.token)
@@ -326,10 +328,10 @@ def exampleParse1 [p: Parser m Token] [MonadExcept String m] [Monad m]: m Unit :
 
 def exampleParse [p: Parser m Token] [MonadExcept String m] [Monad m]: m Unit := do
   assertEq (← p.next) Hint.enter -- enter blogpost
-  assertEq (← p.next) Hint.value; assertEq (← p.token) (Token.string "author")
+  assertEq (← p.next) Hint.value; assertEq (← p.token) (string "author")
   _ ← p.skip                     -- skip author's children, username, ...
-  assertEq (← p.next) Hint.value; assertEq (← p.token) (Token.string "content")
-  assertEq (← p.next) Hint.enter; assertEq (← p.next) Hint.leave -- empty content
+  assertEq (← p.next) Hint.value; assertEq (← p.token) (string "content")
+  assertEq (← p.next) Hint.enter; assertEq (← p.next) Hint.leave
   assertEq (← p.next) Hint.leave -- leave blogpost
   assertEq (← p.next) Hint.eof
 
