VerifiedFilter/Pred/AnyEq.lean
@@ -8,9 +8,8 @@ def Pred.eval {α: Type} [DecidableEq α] (p: Pred α) (x: α): Prop := match p 
   | Pred.eq y => x = y
   | Pred.any => True
 
-def Pred.evalb {α: Type} [DecidableEq α] (p: Pred α) (x: α): Bool := match p with
-  | Pred.eq y => x = y
-  | Pred.any => true
+def Pred.evalb {α: Type} [DecidableEq α] (p: Pred α) (x: α): Bool :=
+  match p with | Pred.eq y => x = y | Pred.any => true
 
 def Pred.evalmb [Monad m] [MonadExcept String m] {α: Type} [DecidableEq α] (p: Pred α) (x: m α): m Bool := do
   match p with
